code/bignum/interfaces/Hacl.Bignum.Crecip.fsti
@@ -7,11 +7,16 @@ open FStar.Buffer
 open Hacl.Bignum.Parameters
 open Hacl.Spec.Bignum.Bigint
 open Hacl.Bignum.Limb
+open Hacl.Spec.Bignum.Crecip
 
 module U32 = FStar.UInt32
+
 
 val crecip:
   out:felem ->
   z:felem -> Stack unit
-  (requires (fun h -> live h out /\ live h z))
-  (ensures (fun h0 _ h1 -> live h1 out /\ modifies_1 out h0 h1))
+  (requires (fun h -> live h out /\ live h z /\ crecip_pre (as_seq h z)))
+  (ensures (fun h0 _ h1 -> live h1 out /\ modifies_1 out h0 h1 /\ live h0 z
+    /\ crecip_pre (as_seq h0 z)
+    /\ as_seq h1 out == crecip_tot (as_seq h0 z)
+  ))
