code/bignum/interfaces/Hacl.Spec.Bignum.Crecip.fsti
@@ -1,0 +1,11 @@
+module Hacl.Spec.Bignum.Crecip
+
+
+open Hacl.Bignum.Parameters
+open Hacl.Spec.Bignum.Bigint
+open Hacl.Bignum.Limb
+
+
+val crecip_pre: s:seqelem -> GTot Type
+
+val crecip_tot: s:seqelem{crecip_pre s} -> Tot (s':seqelem{crecip_pre s'})
